Add first sketches of Paillier (encrypt)

code/experimental/rsapss/Hacl.Impl.Bignum.Comparison.fst
@@ -98,8 +98,7 @@ val bn_is_equal:
   -> Stack bool
     (requires fun h -> live h a /\ live h b)
     (ensures  fun h0 r h1 ->
-     modifies loc_none h0 h1 /\ h0 == h1 /\
-     r == (as_snat h0 a = as_snat h0 b))
+     h0 == h1 /\ r == (as_snat h0 a = as_snat h0 b))
 let bn_is_equal #aLen #bLen a b =
   let res = bn_is_equal_ a b (max' aLen bLen) in
   let h = FStar.HyperStack.ST.get () in
@@ -131,3 +130,31 @@ val bn_is_geq:
      modifies loc_none h0 h1 /\ h0 == h1 /\
      r == (as_snat h0 a >= as_snat h0 b))
 let bn_is_geq #aLen #bLen a b = bn_is_leq b a
+
+
+val bn_is_zero_:
+     #aLen:bn_len
+  -> a:lbignum aLen
+  -> i:size_t{v i <= v aLen}
+  -> Stack bool
+    (requires fun h -> live h a)
+    (ensures  fun h0 _ h1 -> h0 == h1)
+let rec bn_is_zero_ #aLen a i =
+  if i =. 0ul then true else begin
+    let i = i -. 1ul in
+    if not (eq_u64 (a.(i)) (uint 0)) then false
+    else bn_is_zero_ a i
+  end
+
+val bn_is_zero:
+     #aLen:bn_len
+  -> a:lbignum aLen
+  -> Stack bool
+    (requires fun h -> live h a)
+    (ensures fun h0 r h1 ->
+     h0 == h1 /\ r == (as_snat h0 a = 0))
+let bn_is_zero #aLen a =
+  let res = bn_is_zero_ a aLen in
+  let h = FStar.HyperStack.ST.get () in
+  assume (res == (as_snat h a = 0));
+  res
