code/experimental/he/Hacl.Impl.HE.Paillier.fst
@@ -1,0 +1,188 @@
+module Hacl.Impl.HE.Paillier
+
+open FStar.HyperStack
+open FStar.HyperStack.ST
+open FStar.Mul
+
+open LowStar.Buffer
+
+open Lib.IntTypes
+open Lib.Buffer
+open Lib.Math.Algebra
+
+open Hacl.Impl.Bignum
+
+module S = Hacl.Spec.HE.Paillier
+
+
+// max 2^30 bits
+type bn_len_s = s:bn_len{v s <= pow2 22}
+
+val bn_len_s_fits: (l:bn_len_s) -> Lemma
+  (v l * 64 < max_size_t /\
+   v l * 128 < max_size_t /\
+   (v l + 1) < max_size_t
+  )
+let bn_len_s_fits _ = ()
+
+
+#reset-options "--z3rlimit 100 --max_fuel 1 --max_ifuel 0"
+
+type encf_cond (n2Len:bn_len_s) h (n:lbignum n2Len) (n2:lbignum n2Len)
+                (g:lbignum n2Len) (x:lbignum n2Len) (y:lbignum n2Len) =
+       as_snat h n > 1 /\
+       iscomp (as_snat h n) /\
+       as_snat h n * as_snat h n = as_snat h n2 /\
+
+       as_snat h g < as_snat h n2 /\
+       S.is_g (as_snat h n) (as_snat h g) /\
+
+       as_snat h x < as_snat h n /\
+
+       as_snat h y < as_snat h n /\
+       isunit #(as_snat h n) (as_snat h y)
+
+
+val encf:
+     #n2Len:bn_len_s
+  -> n:lbignum n2Len
+  -> n2:lbignum n2Len
+  -> g:lbignum n2Len
+  -> x:lbignum n2Len
+  -> y:lbignum n2Len
+  -> res:lbignum n2Len
+  -> Stack unit
+    (requires fun h ->
+       live h n /\ live h n2 /\ live h g /\ live h x /\ live h y /\ live h res /\
+       all_disjoint [loc n; loc n2; loc g; loc x; loc y; loc res] /\
+       encf_cond n2Len h n n2 g x y
+       )
+    (ensures fun h0 _ h1 ->
+      modifies1 res h0 h1 /\
+      live h1 n /\ live h1 n2 /\ live h1 g /\ live h1 x /\ live h1 y /\
+      (as_snat h1 res = S.encf #(as_snat h0 n) (as_snat h0 g) (as_snat h0 x) (as_snat h0 y))
+      )
+let encf #n2Len n n2 g x y res =
+  bn_len_s_fits n2Len;
+  push_frame();
+  let tmp1:lbignum n2Len = create n2Len (uint 0) in
+  let tmp2:lbignum n2Len = create n2Len (uint 0) in
+  bn_modular_exp n2 g x tmp1;
+  bn_modular_exp n2 y n tmp2;
+  bn_modular_mul n2 tmp1 tmp2 res;
+
+  let h = FStar.HyperStack.ST.get () in
+  to_fe_idemp #(as_snat h n2) (as_snat h g);
+  S.fenu_to_fen2u_lemma #(as_snat h n) (as_snat h y);
+  to_fe_idemp #(as_snat h n2) (as_snat h y);
+
+  pop_frame ()
+
+val encrypt:
+     #n2Len:bn_len_s
+  -> n:lbignum n2Len
+  -> n2:lbignum n2Len
+  -> g:lbignum n2Len
+  -> r:lbignum n2Len
+  -> m:lbignum n2Len
+  -> res:lbignum n2Len
+  -> Stack unit
+    (requires fun h ->
+       live h n /\ live h n2 /\ live h g /\ live h r /\ live h m /\ live h res /\
+       all_disjoint [loc n; loc n2; loc g; loc r; loc m; loc res] /\
+       encf_cond n2Len h n n2 g m r
+       )
+    (ensures fun h0 _ h1 -> true)
+let encrypt #n2Len n n2 g r m res = encf n n2 g m r res
+
+val bigl:
+     #len:bn_len_s
+  -> n:lbignum len
+  -> u:lbignum len
+  -> res:lbignum len
+  -> Stack unit
+    (requires fun h ->
+     live h n /\ live h u /\ live h res /\
+     as_snat h n > 1 /\
+     as_snat h u > 0 /\
+     as_snat h u < as_snat h n /\
+     iscomp (as_snat h n) /\
+     isunit #(as_snat h n) (as_snat h u))
+    (ensures fun h0 _ h1 ->
+     live h1 n /\ live h1 u /\
+     modifies1 res h0 h1 /\
+     as_snat h1 res = S.bigl #(as_snat h0 n) (as_snat h0 u)
+     )
+let bigl #len n u res = admit() // requires bignum division
+
+
+type l1_div_l2_cond h (n2Len:bn_len_s) (p:lbignum n2Len) (q:lbignum n2Len)
+                      (n:lbignum n2Len) (n2:lbignum n2Len) (w:lbignum n2Len)
+                      (g:lbignum n2Len) (lambda:lbignum n2Len) (l2inv:lbignum n2Len) =
+       (let n = as_snat h n in
+        let n2 = as_snat h n2 in
+        let g = as_snat h g in
+        let lambda = as_snat h lambda in
+       (as_snat h p > 1 /\ as_snat h q > 1 /\ n > 1 /\
+        isprm (as_snat h p) /\ isprm (as_snat h q) /\
+        n = as_snat h p * as_snat h q /\
+        n > 1 /\
+        iscomp n /\
+        n2 > 1 /\
+        n2 = n * n /\
+
+        as_snat h w < n /\
+        as_snat h w < n2 /\ // todo remove
+
+        g < n2 /\
+        S.is_g n g /\
+
+        lambda = S.etot (as_snat h p) (as_snat h q) /\
+        lambda < n2 /\
+
+        (let x:S.fen2 n = fexp #n2 g lambda in
+         assert (isunit #n2 g);
+         g_pow_isunit #n2 g lambda;
+         isunit_nonzero x;
+         as_snat h l2inv = finv0 #n (S.bigl #n x))
+        ))
+
+
+#reset-options "--z3rlimit 100 --max_fuel 1 --max_ifuel 0"
+
+
+val l1_div_l2:
+     #n2Len:bn_len_s
+  -> p:lbignum n2Len
+  -> q:lbignum n2Len
+  -> n:lbignum n2Len
+  -> n2:lbignum n2Len
+  -> w:lbignum n2Len
+  -> g:lbignum n2Len
+  -> lambda:lbignum n2Len
+  -> l2inv:lbignum n2Len
+  -> res:lbignum n2Len
+  -> Stack unit
+    (requires fun h ->
+       live h p /\ live h q /\ live h n /\ live h w /\ live h g /\
+       live h lambda /\ live h l2inv /\ live h res /\
+       all_disjoint [loc p; loc q; loc n; loc w; loc g; loc l2inv; loc res] /\
+       l1_div_l2_cond h n2Len p q n n2 w g lambda l2inv
+       )
+    (ensures fun h0 _ h1 ->
+       live h1 p /\ live h1 q /\ live h1 n /\ live h1 w /\
+       live h1 g /\ live h1 lambda /\ live h1 l2inv /\
+       modifies1 res h0 h1
+
+    )
+let l1_div_l2 #n2Len p q n n2 w g lambda l2inv res =
+  push_frame ();
+
+  let l1arg:lbignum n2Len = create n2Len (uint 0) in
+  //bn_modular_exp n2 w lambda l1arg;
+
+  //if bn_is_zero l1arg then bn_assign_uint64 res 0uL;
+
+  admit();
+
+  pop_frame ()
